AcornExamples.v
@@ -149,8 +149,11 @@ Module AcornListBase.
     induction l;simpl;congruence.
   Qed.
 
+  Arguments foldr {_ _}.
+  Arguments concat {_}.
+
   Lemma oak_foldr_coq_fold_right (A B : Set) (l : OakList A) (f : A -> B -> B) a :
-    foldr _ _  f a l = fold_right f a (from_oak l).
+    foldr f a l = fold_right f a (from_oak l).
   Proof.
     induction l;simpl;auto.
     f_equal. congruence.
@@ -159,7 +162,7 @@ Module AcornListBase.
   Open Scope list.
 
   Lemma concat_app (A : Set) (l1 l2 : OakList A) :
-  concat _ l1 l2 = to_oak (from_oak l1 ++ from_oak l2).
+  concat l1 l2 = to_oak (from_oak l1 ++ from_oak l2).
   Proof.
     revert l2.
     induction l1;intros l2;destruct l2;simpl;try rewrite to_from_oak;auto.
@@ -172,19 +175,15 @@ Module AcornListBase.
   Hint Rewrite oak_foldr_coq_fold_right concat_app from_to_oak : hints.
 
   Lemma concat_assoc :
-    forall (A : Set) (l m n : OakList A), concat _ l (concat _ m n) = concat _ (concat _ l m) n.
+    forall (A : Set) (l m n : OakList A), concat l (concat m n) = concat (concat l m) n.
   Proof.
     intros. autorewrite with hints. f_equal.
     apply app_assoc.
   Qed.
 
-  Lemma foldr_concat :
-    forall (A B : Set) (f : A -> B -> B) (l l' : OakList A) (i : B),
-      foldr _ _ f i (concat _ l l') = foldr _ _ f (foldr _ _ f i l') l.
-  Proof.
-    intros. autorewrite with hints.
-    apply fold_right_app.
-  Qed.
+  Lemma foldr_concat (A B : Set) (f : A -> B -> B) (l l' : OakList A) (i : B) :
+      foldr f i (concat l l') = foldr f (foldr f i l') l.
+  Proof. autorewrite with hints;apply fold_right_app. Qed.
 
 End AcornListBase.
 
